WIP on AEAD testing

examples/low-level/crypto/Plain.fst
@@ -28,16 +28,34 @@ type buffer = Buffer.buffer UInt8.t
 type lbytes (l:nat)  = b:bytes  {Seq.length b = l}
 type lbuffer (l:nat) = b:buffer {Buffer.length b = l}
 
-assume val sel_bytes: h:mem -> l:UInt32.t -> buf:lbuffer(v l){Buffer.live h buf}  -> Tot (lbytes (v l))
+val sel_bytes: h:mem -> l:UInt32.t -> buf:lbuffer(v l){Buffer.live h buf}  -> GTot (lbytes (v l))
+let rec sel_bytes h l buf = Buffer.as_seq h buf
 
-//TODO add functional correctness
-assume val load_bytes: l:UInt32.t -> buf:lbuffer(v l) -> Stack (lbytes(v l))
+val load_bytes: l:UInt32.t -> buf:lbuffer(v l) -> Stack (lbytes(v l))
   (requires (fun h0 -> Buffer.live h0 buf))
   (ensures (fun h0 r h1 -> h0 == h1 /\ Buffer.live h0 buf /\ r == sel_bytes h1 l buf))
-assume val store_bytes: l:UInt32.t -> buf:lbuffer(v l) -> b:lbytes(v l) -> ST unit
+let rec load_bytes l buf = 
+  assume false;//16-09-21 TODO 
+  if l = 0ul then Seq.createEmpty else
+  let b = Buffer.index buf 0ul in
+  let t = load_bytes (l -^ 1ul) (Buffer.sub buf 1ul (l -^ 1ul)) in
+  SeqProperties.cons b t
+
+val store_bytes: l:UInt32.t -> buf:lbuffer(v l) -> b:lbytes(v l) -> ST unit
   (requires (fun h0 -> Buffer.live h0 buf))
   (ensures (fun h0 r h1 -> Buffer.live h1 buf /\ modifies_1 buf h0 h1 /\ b == sel_bytes h1 l buf
   ))
+
+val store_bytes_aux: len:UInt32.t -> buf:lbuffer(v len) -> i:UInt32.t  {i <=^ len} -> b:lbytes(v len) -> ST unit
+  (requires (fun h0 -> Buffer.live h0 buf))
+  (ensures (fun h0 r h1 -> Buffer.live h1 buf /\ modifies_1 buf h0 h1 /\ b == sel_bytes h1 len buf
+  ))
+let rec store_bytes_aux len buf i b = 
+  assume false;//16-09-21 TODO 
+  if i <^ len then (
+  Buffer.upd buf i (Seq.index b (v i));
+  store_bytes_aux len buf (i +^ 1ul) b)
+let store_bytes l buf b = store_bytes_aux l buf 0ul b
 
 // SECRETS, HIGH AND LOW
 
@@ -105,7 +123,7 @@ val bufferRepr: #i:id {~(authId i)} -> #l:plainLen -> b:plainBuffer i l -> Tot (
 let bufferRepr #i #l b = b
 // not sure how to write modifies clauses including plain and plainBuffer
 
-val sel_plain: h:mem -> #i:id -> l:UInt32.t -> buf:plainBuffer i (v l){live h buf} -> Tot (plain i (v l)) 
+val sel_plain: h:mem -> #i:id -> l:UInt32.t -> buf:plainBuffer i (v l){live h buf} -> GTot (plain i (v l)) 
 let sel_plain h #i l buf = sel_bytes h l buf
 
 val load: #i:id -> l:UInt32.t -> buf: plainBuffer i (v l) -> ST (plain i (v l)) 
